{
    "cells": [
        {
            "cell_type": "markdown",
            "id": "0",
            "metadata": {},
            "source": [
                "# \u5f62\u5f0f\u5e42\u7ea7\u6570\n",
                "\n",
                "$\\sum_{i=0}^{\\infty}{x^i}=\\frac{1}{1-x}$\n",
                "\n",
                "$\\sum_{i=0}^{\\infty}{a^ix^i}=\\frac{1}{1-ax}$\n",
                "\n",
                "$\\sum_{i=0}^{\\infty}{x^{ik}}=\\frac{1}{1-x^k}$\n",
                "\n",
                "$\\sum_{i=0}^{\\infty}{c^ix^{ik}}=\\frac{1}{1-cx^k}$\n",
                "\n",
                "$\\sum_{i=0}^{\\infty}{\\frac{x^i}{i!}}=e^x$\n",
                "\n",
                "$x\\frac{\\partial}{\\partial{x}}\\sum_{i=0}^{\\infty}{a_ix^i}=\\sum_{i=0}^{\\infty}{ia_ix^i}$\n",
                "\n",
                "$\\sum_{i=0}^{n}{\\binom{n}{i}(-x)^i}=(1-x)^n$\n",
                "\n",
                "$\\sum_{i=0}^{\\infty}{\\binom{n+i}{i}x^i}=\\frac{1}{(1-x)^{n+1}}$\n",
                "\n",
                "\u5e73\u79fb: $[x^n]x^tF(x)=F[n-t]$\n",
                "\n",
                "\u62c9\u4f38: $F(x^k)=\\sum_{i=0}^{\\infty}{F[i]x^{ik}}$\n",
                "\n",
                "$\\sum_{i=0}^{\\infty}{\\frac{a^{\\underline{i}}}{i!}x^i}=(1+x)^a$\n",
                "\n",
                "$ln(\\frac{1}{1-x})=\\sum_{i=1}^{\\infty}{\\frac{x^i}{i}}$\n",
                "\n",
                "$ln(F(x))=-\\sum_{i=1}^{\\infty}{\\frac{(1-F(x))^i}{i}}$\n",
                "\n",
                "$e^{F(x)}=\\sum_{i=0}^{\\infty}{\\frac{F(x)^i}{i!}}$\n",
                "\n",
                "\n",
                "## \u4e00\u4e9b\u7279\u6b8a\u60c5\u5f62\u4e0b EGF \u4e0e OGF \u7684\u8f6c\u5316\n",
                "\n",
                "\u9996\u5148\u5b9a\u4e49 $F_{exp}(x)=\\sum_{i=0}^{\\infty}\\frac{f_ix^i}{i!}$ \u548c $F(x)=\\sum_{i=0}^{\\infty}f_ix^i$.\n",
                "\n",
                "\u4ee5\u4e0b\u5f0f\u5b50\u5e38\u7528\u4e8e\u5df2\u77e5EGF\u8868\u793a, \u9700\u8981\u6c42OGF\u8868\u793a(\u6216\u53cd\u8fc7\u6765)\u7684\u573a\u5408.\n",
                "\n",
                "$F_{exp}(x)=\\sum_{i}A_ie^{C_ix}\\Leftrightarrow F(x)=\\sum_{i}\\frac{A_i}{1-C_ix}$.\n",
                "\n",
                "$F_{exp}(x)=\\sum_{i}x^{D_i}e^{C_ix}\\Leftrightarrow F(x)=\\sum_{i}\\frac{D_i!x^{D_i}}{(1-C_ix)^{D_i+1}}$.\n",
                "\n",
                "\n",
                "## Taylor shift\n",
                "[source](https://codeforces.com/blog/entry/99646)\n",
                "\n",
                "\u6cf0\u52d2\u5c55\u5f00\u7684\u7b97\u5b50\u5f62\u5f0f: $e^{tD}F(x)=F(x+t)$, \u5176\u4e2d $D=\\frac{d}{dx}$, $F(x)$ \u4e3a\u5f62\u5f0f\u5e42\u7ea7\u6570(\u5b9e\u9645\u4e0a, \u6761\u4ef6\u4e3a\u89e3\u6790\u51fd\u6570).\n",
                "\n",
                "\u5b9a\u4e49\u5f62\u5f0f\u5e42\u7ea7\u6570\u73af\u4e0a\u7684\u4e24\u4e2a\u7ebf\u6027\u7b97\u5b50:\n",
                "\n",
                "Borel \u7b97\u5b50: $\\mathcal{B}(x^i)=\\frac{x^i}{i!}$.\n",
                "\n",
                "Laplace \u7b97\u5b50: $\\mathcal{L}(x^i)=i!x^i$.\n",
                "\n",
                "\u5bb9\u6613\u770b\u51fa\u6709 $\\mathcal{B}(\\mathcal{L}(F(x)))=\\mathcal{L}(\\mathcal{B}(F(x)))=F(x)$ \u6210\u7acb.\n",
                "\n",
                "\u53e6\u4e00\u4e2a\u91cd\u8981\u7684\u89c2\u5bdf\u662f,\n",
                "\n",
                "$$D^i\\mathcal{B}(x^j)=\\frac{x^{j-i}}{(j-i)!}=\\mathcal{B}(x^{j-i}),$$\n",
                "\n",
                "\u6cdb\u5316\u53ef\u5f97:\n",
                "\n",
                "$$D^i\\mathcal{B}(F(x))=\\mathcal{B}(x^{-i}F(x))$$\n",
                "\n",
                "\u5bf9\u4efb\u610f\u7684\u5f62\u5f0f\u5e42\u7ea7\u6570 $F(x)$ \u6210\u7acb. \u8fd9\u91cc\u6211\u4eec\u5b9a\u4e49 \u5bf9\u4e8e\u6240\u6709\u7684 $i\\gt j$ \u6709 $(j-i)!=\\infty$. \u56e0\u6b64\u6709 $\\mathcal{B}(x^k)=0,\\forall k\\lt 0$.\n",
                "\n",
                "\u7531\u4e8eBorel\u7b97\u5b50\u7684\u7ebf\u6027\u6027, \u53ef\u4ee5\u66f4\u8fdb\u4e00\u6b65\u6cdb\u5316\u5f97\u5230:\n",
                "\n",
                "$$G(D)\\mathcal{B}(F(x))=\\mathcal{B}(G(x^{-1})F(x))$$\n",
                "\u5bf9\u4efb\u610f\u7684\u5f62\u5f0f\u5e42\u7ea7\u6570 $F(x)$ \u548c $G(x)$ \u6210\u7acb.\n",
                "\n",
                "\u7ed3\u5408\u7b2c\u4e00\u6761\u6027\u8d28\u4ee5\u53ca\u6cf0\u52d2\u5c55\u5f00, \u6211\u4eec\u5f97\u5230:\n",
                "\n",
                "$$F(x+a)=e^{aD}F(x)=e^{aD}\\mathcal{B}(\\mathcal{L}(F(x)))=\\mathcal{B}(e^{ax^{-1}}\\mathcal{L}(F(x))).$$"
            ]
        }
    ],
    "metadata": {},
    "nbformat": 4,
    "nbformat_minor": 5
}