{"cells": [{"cell_type": "markdown", "id": "0", "metadata": {}, "source": ["# \u5fae\u79ef\u5206\u57fa\u7840\n", "\n", "\u6c42\u5bfc\u7684\u7ebf\u6027\u6027:\n", "\n", "$(F(x)+G(x))'=F'(x)+G'(x)$\n", "\n", "$(c \\cdot F(x))'=c \\cdot F'(x)$\n", "\n", "\u90e8\u5206\u521d\u7b49\u51fd\u6570\u7684\u5bfc\u6570:\n", "\n", "$(C)'=0$\n", "\n", "$(x^k)'=kx^{k-1}$\n", "\n", "$(e^x)'=e^x$\n", "\n", "$(a^x)'=a^x\\ln(a)$\n", "\n", "$(\\ln(x))'=\\frac{1}{x}$\n", "\n", "$(\\log_a(x))'=\\frac{1}{x\\ln(a)}$\n", "\n", "$(\\sin(x))'=\\cos(x)$\n", "\n", "$(\\cos(x))'=-\\sin(x)$\n", "\n", "\u4e58\u6cd5\u6cd5\u5219: $(F(x)G(x))'=F'(x)G(x)+F(x)G'(x)$\n", "\n", "\u9664\u6cd5\u6cd5\u5219: $(\\frac{F(x)}{G(x)})'=\\frac{F'(x)G(x)-F(x)G'(x)}{G^2(x)}$\n", "\n", "\u83b1\u5e03\u5c3c\u5179\u516c\u5f0f: $(\\frac{d}{dx})^k(F(x) \\cdot G(x))=\\sum_{i=0}^{k}{\\binom{k}{i}(\\frac{d}{dx})^iF(x)(\\frac{d}{dx})^{k-i}G(x)}$\n", "\n", "\u94fe\u5f0f\u6cd5\u5219: $\\frac{dy}{dx}\\frac{d}{dy}=\\frac{d}{dx}$\n", "\n", "\u504f\u5bfc\u6570\u94fe\u5f0f\u6cd5\u5219: \u753b\u51fa\u53d8\u91cf\u7684DAG, \u5bf9\u6240\u6709\u8def\u5f84\u6c42\u548c\n", "\n", "\u590d\u5408\u51fd\u6570\u6c42\u5bfc: $(G(F(x)))'=G'(F(x))F'(x)$\n", "\n", "\u5373 $\\frac{d}{dx}G(F(x))=\\frac{dF(x)}{dx}\\frac{d}{dF(x)}G(F(x))=G'(F(x))F'(x)$\n", "\n", "\u53cd\u51fd\u6570(\u590d\u5408\u9006)\u6c42\u5bfc: $F(x)$\u7684\u53cd\u51fd\u6570$G(x)$\u7684\u5bfc\u6570\u4e3a$\\frac{1}{F'(x)}$, \u6216\u5199\u4f5c$\\frac{dx}{dy}=\\frac{1}{\\frac{dy}{dx}}$\n", "\n", "\u79ef\u5206\u7684\u7ebf\u6027\u6027:\n", "\n", "$\\int(F(x)+G(x))dx=\\int{F(x)dx}+\\int{G(x)dx}$\n", "\n", "$\\int{cF(x)dx}=c\\int{F(x)dx}$\n", "\n", "\u79ef\u5206\u4e2d\u7684\u94fe\u5f0f\u6cd5\u5219: $\\int{G'(F(x))F'(x)dx}=G(F(x))+C$, \u5373\u9006\u7528\u6c42\u5bfc\u7684\u94fe\u5f0f\u6cd5\u5219\n", "\n", "\u5206\u6b65\u79ef\u5206\u6cd5: \u7531$(F(x)G(x))'=F'(x)G(x)+F(x)G'(x)$\u79fb\u9879\u5e76\u4e24\u8fb9\u79ef\u5206\u5f97$\\int{F'(x)G(x)dx}=F(x)G(x)-\\int{F(x)G'(x)dx}$\n", "\n", "\u6cf0\u52d2\u5c55\u5f00: $F(x)=\\sum_{i=0}^{\\infty}{\\frac{F^{(i)}(a)}{i!}(x-a)^i}$\n", "\n", "\u9ea6\u514b\u52b3\u6797\u7ea7\u6570: \u5728$x=0$\u5904\u4f5c\u6cf0\u52d2\u5c55\u5f00, $F(x)=\\sum_{i=0}^{\\infty}{\\frac{F^{(i)}(0)}{i!}x^i}$"]}], "metadata": {}, "nbformat": 4, "nbformat_minor": 5}