{"cells": [{"cell_type": "markdown", "id": "0", "metadata": {}, "source": ["# \u53cd\u6f14\n", "\n", "\u672c\u8d28\u4e0a\u662f\u6c42\u9006.\n", "\n", "## Formulation\n", "\n", "Assume that $f[n] = \\sum_{i}{a_{n,i}g[i]}$. Given $f$, find $g$.\n", "\n", "## Framework of prove\n", "\n", "Assume $Ax=b$, given $b$, find $x$.\n", "\n", "At the first step, we find some $B$ s.t. $BA=I$, then:\n", "\n", "$x=Ix\\iff\\\\\n", "x=(BA)x\\iff\\\\\n", "x=B(Ax)\\iff\\\\\n", "x=Bb\\\\\n", "Q.E.D.$\n", "\n", "## \u4e8c\u9879\u5f0f\u53cd\u6f14\n", "\n", "### Core formula\n", "\n", "$(1 - 1)^n = \\sum_{i=0}^{n}{\\binom{n}{i}(-1)^i} = [n = 0]$\n", "\n", "where $[n = 0]$ means $1$ if $n$ is zero, otherwise $0$.\n", "\n", "Given $f[n] = \\sum_{i=0}^{n}{\\binom{n}{i}g[i]}$, we have:\n", "\n", "$g[n] = \\sum_{i=0}^{n}{\\binom{n}{i}(-1)^{n-i}f[i]}$.\n", "\n", "### Prove\n", "\n", "$g[n] = \\sum_{m=0}^{n}{\\binom{n}{m}[n-m=0]g[m]}\\iff\\\\\n", "g[n] = \\sum_{m=0}^{n}{\\binom{n}{m}\\sum_{i=0}^{n-m}{\\binom{n-m}{i}(-1)^{i}g[m]}}\\iff\\\\\n", "g[n] = \\sum_{i=0}^{n}{\\binom{n}{i}(-1)^i\\sum_{m=0}^{n-i}{\\binom{n-i}{m}g[m]}}\\iff\\\\\n", "g[n] = \\sum_{i=0}^{n}{\\binom{n}{i}(-1)^if[n-i]}\\iff\\\\\n", "g[n] = \\sum_{i=0}^{n}{\\binom{n}{n-i}(-1)^{n-i}f[i]}\\\\\n", "Q.E.D.$\n", "\n", "## \u83ab\u6bd4\u4e4c\u65af\u53cd\u6f14\n", "\n", "### Core formula\n", "\n", "$\\sum_{d|n}\\mu(d)=[n=1]$.\n", "\n", "Given $f[n] = \\sum_{d|n}g[d]$, we have:\n", "\n", "$g[n] = \\sum_{d|n}\\mu(\\frac{n}{d})f[d]$.\n", "\n", "### Prove\n", "\n", "$g[n] = \\sum_{m|n}[\\frac{n}{m}=1]g[m]\\iff\\\\\n", "g[n] = \\sum_{m|n}\\sum_{d|\\frac{n}{m}}\\mu(d)g[m]\\iff\\\\\n", "g[n] = \\sum_{d|n}\\mu(d)\\sum_{m|\\frac{n}{d}}g[m]\\iff\\\\\n", "g[n] = \\sum_{d|n}\\mu(d)f[\\frac{n}{d}]\\iff\\\\\n", "g[n] = \\sum_{d|n}\\mu(\\frac{n}{d})f[d]\\\\\n", "Q.E.D.$\n", "\n", "## \u5b50\u96c6\u53cd\u6f14 \n", "\n", "### Core formula\n", "\n", "$\\sum_{T\\subseteq S}(-1)^{|T|}=[S = \\emptyset]$\n", "\n", "Given $f[S] = \\sum_{T\\subseteq S}g[T]$, we have:\n", "\n", "$g[S] = \\sum_{T\\subseteq S}(-1)^{|S|-|T|}f[T]$.\n", "\n", "### Prove\n", "\n", "$g[S] = \\sum_{W\\subseteq S}[S\\setminus W = \\emptyset]g[W]\\iff\\\\\n", "g[S] = \\sum_{W\\subseteq S}\\sum_{T\\subseteq {S\\setminus W}}(-1)^{|T|}g[W]\\iff\\\\\n", "g[S] = \\sum_{T\\subseteq S}(-1)^{|T|}\\sum_{W\\subseteq {S\\setminus T}}g[W]\\iff\\\\\n", "g[S] = \\sum_{T\\subseteq S}(-1)^{|T|}g[S\\setminus T]\\iff\\\\\n", "g[S] = \\sum_{T\\subseteq S}(-1)^{|S|-|T|}g[T]\\\\\n", "Q.E.D.$\n", "\n", "### Applications\n", "\n", "#### A1\n", "\n", "\u5bf9\u4e8e\u4efb\u610f\u7684\u5173\u4e8e\u96c6\u5408$S$\u7684\u51fd\u6570, \u6211\u4eec\u6709:\n", "\n", "$f[S] = \\sum_{T\\subseteq S}\\sum_{P\\subseteq T}(-1)^{|T|-|P|}f(P)$\n", "\n", "##### Prove\n", "\n", "$RHS = \\sum_{P\\subseteq S}f[P]\\sum_{P\\subseteq T \\subseteq S}(-1)^{|T|-|P|}$\n", "\n", "$RHS = \\sum_{P\\subseteq S}f[P]\\sum_{i=0}^{|S|-|P|}\\binom{|S|-|P|}{i}(-1)^{i}$\n", "\n", "$RHS = \\sum_{P\\subseteq S}f[P](1 - 1)^{|S|-|P|}$\n", "\n", "$RHS = f[S] = LHS$\n", "\n", "$Q.E.D.$\n", "\n", "##### \u76f8\u5173\u9898\u76ee\n", "\n", "https://www.luogu.com.cn/problem/P5206\n", "\n", "## \u5355\u4f4d\u6839\u53cd\u6f14\n", "\n", "### Core formula\n", "\n", "$\\omega_n$: $n$\u6b21\u5355\u4f4d\u6839 s.t. $\\omega_n^n=1$ (e.g. \u590d\u6570\u57df\u4e0a\u7684$e^{\\frac{2\\pi i}{n}}$).\n", "\n", "$\\frac{1}{n}\\sum_{k=0}^{n-1}\\omega_n^{vk} = [v\\equiv 0\\mod n]$\n", "\n", "Given $f[m]=\\sum_{k=0}^{n-1}\\omega_n^{mk}g[k]$, we have:\n", "\n", "$g[m]=\\frac{1}{n}\\sum_{k=0}^{n-1}\\omega_n^{-mk}f[k]$.\n", "\n", "### Applications\n", "\n", "$[p+q\\equiv r \\mod n]\\iff\\\\\n", "[p+q-r\\equiv 0 \\mod n]\\iff\\\\\n", "\\frac{1}{n}\\sum_{k=0}^{n-1}\\omega_n^{(p+q-r)k}\\iff\\\\\n", "\\frac{1}{n}\\sum_{k=0}^{n-1}\\omega_n^{-rk}\\omega_n^{pk}\\omega_n^{qk}$\n", "\n", "at where $p,q,r$ looks more independent.\n", "\n", "# Reference\n", "[\u70ab\u9177\u53cd\u6f14\u9b54\u672f](https://vfleaking.blog.uoj.ac/blog/87)"]}], "metadata": {}, "nbformat": 4, "nbformat_minor": 5}