{"cells": [{"cell_type": "markdown", "id": "0", "metadata": {}, "source": ["# \u725b\u987f\u6052\u7b49\u5f0f\n", "\n", "https://en.wikipedia.org/wiki/Newton%27s_identities\n", "\n", "## Elementary symmetric polynomial\n", "\n", "https://en.wikipedia.org/wiki/Elementary_symmetric_polynomial\n", "\n", "### Definition\n", "\n", "The elementary symmetric polynomials in $n$ variables $x_1, x_2, ..., x_n$, written $e_k(x_1,x_2,...,x_n)$ for $k=0,1,2,...,n$, are defined by\n", "\n", "$e_0(x_1,x_2,...,x_n)=1$,\n", "\n", "$e_1(x_1,x_2,...,x_n)=\\sum_{1\\leq j\\leq n}{x_j}$,\n", "\n", "$e_2(x_1,x_2,...,x_n)=\\sum_{1\\leq j\\lt k\\leq n}{x_jx_k}$,\n", "\n", "$e_3(x_1,x_2,...,x_n)=\\sum_{1\\leq j\\lt k\\lt l\\leq n}{x_jx_kx_l}$,\n", "\n", "$...$\n", "\n", "$e_k(x_1,x_2,...,x_n)=\\sum_{1\\leq j_1\\lt j_2\\lt ...\\lt j_k\\leq n}{x_{j_1}x_{j_2}...x_{j_k}}$,\n", "\n", "so that $e_k(x_1,x_2,...,x_n)=0$ if $k\\gt n$.\n", "\n", "### Properties\n", "\n", "$\\Pi_{j=1}^{n}{(\\lambda-x_j)}=\\lambda^n-e_1(x_1,x_2,...,x_n)\\lambda^{n-1}+e_2(x_1,x_2,...,x_n)\\lambda^{n-2}+...+(-1)^ne_n(x_1,x_2,...,x_n)=\\sum_{i=0}^{n}{(-1)^ie_i(x_1,x_2,...,x_n)\\lambda^{n-i}}$\n", "\n", "## Complete homogeneous symmetric polynomial\n", "\n", "https://en.wikipedia.org/wiki/Complete_homogeneous_symmetric_polynomial\n", "\n", "### Definition\n", "\n", "The complete homogeneous symmetric polynomial of degree $k$ in $n$ variables $x_1,x_2,...,x_n$, written $h_k$ for $k=0,1,2,...$, is the sum of all monomials of total degree $k$ in the variables.\n", "\n", "Formally,\n", "\n", "$h_k(x_1,x_2,...,x_n)=\\sum_{1\\leq j_1\\leq j_2\\leq...\\leq j_k \\leq n}{x_{j_1}x_{j_2}...x_{j_k}}$.\n", "\n", "The formula can also be written as:\n", "\n", "$h_k(x_1,x_2,...x_n)=\\sum_{l_1+l_2+...+l_n=k,l_i\\geq 0}{x_1^{l_1}x_2^{l_2}...x_n^{l_n}}$.\n", "\n", "Yet another form:\n", "\n", "$h_k(x_1,x_2,...,x_n)=\\sum_{1\\leq j_1,j_2,...,j_k\\leq n}{\\frac{m_1!m_2!...m_n!}{k!}x_{j_1}x_{j_2}...x_{j_k}}$,\n", "\n", "here $m_p$ is the multiplicity of number $p$ in the sequence ${j_1,j_2,...,j_k}$.\n", "\n", "### Properties\n", "\n", "#### Generating function\n", "\n", "$\\sum_{k=0}^{\\infty}{h_k(x_1,x_2,...,x_n)t^k}=\\Pi_{i=1}^{n}\\sum_{j=0}^{\\infty}{(x_it)^j}=\\Pi_{i=1}^{n}{\\frac{1}{1-x_it}}$\n", "\n", "#### Relation with the elementary symmetric polynomials\n", "\n", "$\\sum_{i=0}^{m}{(-1)^ie_i(x_1,x_2,...,x_n)h_{m-i}(x_1,x_2,...,x_n)=0}$ for all $m > 0$.\n", "\n", "Proof:\n", "\n", "$\\sum_{k=0}^{\\infty}{e_k(x_1,x_2,...,x_n)(-t)^k}=\\Pi_{i=1}^{n}{(1-x_it)}$,\n", "\n", "$[x^m](\\sum_{k=0}^{\\infty}{e_k(x_1,x_2,...x_n)(-t)^k})(\\sum_{k=0}^{\\infty}{h_k(x_1,x_2,...x_n)t^k})=[x^m](\\Pi_{i=1}^{n}{(1-x_it)})(\\frac{1}{\\Pi_{i=1}^{n}{(1-x_it)}})=[x^m]{(1)}=[m=0]$,\n", "\n", "extract coefficients on both sides for $m\\gt 0$ and the prove done.\n", "\n", "#### Relation with the Stirling numbers\n", "\n", "$h_k(x_1,x_2,...,x_n)=\\begin{Bmatrix}n+k \\\\ n\\end{Bmatrix}$,\n", "\n", "$e_k(x_1,x_2,...,x_n)=\\begin{bmatrix}n+1 \\\\ n+1-k\\end{bmatrix}$.\n", "\n", "#### Relation with power sums\n", "\n", "$kh_k=\\sum_{i=1}^{k}{h_{k-i}p_i}$\n", "\n", "## Power sums\n", "\n", "$p_k(x_1,x_2,...,x_n)=\\sum_{i=1}^{n}{x_i^k}$.\n", "\n", "## Newton's identities\n", "\n", "$ke_k(x_1,x_2,...,x_n)=\\sum_{i=1}^{k}{(-1)^{i-1}e_{k-i}(x_1,x_2,...,x_n)p_i(x_1,x_2,...,x_n)}$, valid for all $n\\geq1$."]}], "metadata": {}, "nbformat": 4, "nbformat_minor": 5}