{
 "cells": [
  {
   "cell_type": "markdown",
   "id": "ae41a41e",
   "metadata": {},
   "source": [
    "# 反演\n",
    "\n",
    "本质上是求逆.\n",
    "\n",
    "## Formulation\n",
    "\n",
    "Assume that $f[n] = \\sum_{i}{a_{n,i}g[i]}$. Given $f$, find $g$.\n",
    "\n",
    "## Framework of prove\n",
    "\n",
    "Assume $Ax=b$, given $b$, find $x$.\n",
    "\n",
    "At the first step, we find some $B$ s.t. $BA=I$, then:\n",
    "\n",
    "$x=Ix\\\\\n",
    "x=(BA)x\\\\\n",
    "x=B(Ax)\\\\\n",
    "x=Bb\\\\\n",
    "Q.E.D.$\n",
    "\n",
    "## 二项式反演\n",
    "\n",
    "### Core formula\n",
    "\n",
    "$(1 - 1)^n = \\sum_{i=0}^{n}{\\binom{n}{i}(-1)^i} = [n = 0]$\n",
    "\n",
    "where $[n = 0]$ means $1$ if $n$ is zero, otherwise $0$.\n",
    "\n",
    "Given $f[n] = \\sum_{i=0}^{n}{\\binom{n}{i}g[i]}$, we have:\n",
    "\n",
    "$g[n] = \\sum_{i=0}^{n}{\\binom{n}{i}(-1)^{n-i}f[i]}$.\n",
    "\n",
    "### Prove\n",
    "\n",
    "$g[n] = \\sum_{m=0}^{n}{\\binom{n}{m}[n-m=0]g[m]}\\\\\n",
    "g[n] = \\sum_{m=0}^{n}{\\binom{n}{m}\\sum_{i=0}^{n-m}{\\binom{n-m}{i}(-1)^{i}g[m]}}\\\\\n",
    "g[n] = \\sum_{i=0}^{n}{\\binom{n}{i}(-1)^i\\sum_{m=0}^{n-i}{\\binom{n-i}{m}g[m]}}\\\\\n",
    "g[n] = \\sum_{i=0}^{n}{\\binom{n}{i}(-1)^if[n-i]}\\\\\n",
    "g[n] = \\sum_{i=0}^{n}{\\binom{n}{n-i}(-1)^{n-i}f[i]}\\\\\n",
    "Q.E.D.$\n",
    "\n",
    "## 莫比乌斯反演\n",
    "\n",
    "### Core formula\n",
    "\n",
    "$\\sum_{d|n}\\mu(d)=[n=1]$.\n",
    "\n",
    "Given $f[n] = \\sum_{d|n}g[d]$, we have:\n",
    "\n",
    "$g[n] = \\sum_{d|n}\\mu(\\frac{n}{d})f[d]$.\n",
    "\n",
    "### Prove\n",
    "\n",
    "$g[n] = \\sum_{m|n}[\\frac{n}{m}=1]g[m]\\\\\n",
    "g[n] = \\sum_{m|n}\\sum_{d|\\frac{n}{m}}\\mu(d)g[m]\\\\\n",
    "g[n] = \\sum_{d|n}\\mu(d)\\sum_{m|\\frac{n}{d}}g[m]\\\\\n",
    "g[n] = \\sum_{d|n}\\mu(d)f[\\frac{n}{d}]\\\\\n",
    "g[n] = \\sum_{d|n}\\mu(\\frac{n}{d})f[d]\\\\\n",
    "Q.E.D.$\n",
    "\n",
    "## 子集反演 \n",
    "\n",
    "### Core formula\n",
    "\n",
    "$\\sum_{T\\subseteq S}(-1)^{|T|}=[S = \\emptyset]$\n",
    "\n",
    "Given $f[S] = \\sum_{T\\subseteq S}g[T]$, we have:\n",
    "\n",
    "$g[S] = \\sum_{T\\subseteq S}(-1)^{|S|-|T|}f[T]$.\n",
    "\n",
    "### Prove\n",
    "\n",
    "$g[S] = \\sum_{W\\subseteq S}[S\\setminus W = \\emptyset]g[W]\\\\\n",
    "g[S] = \\sum_{W\\subseteq S}\\sum_{T\\subseteq {S\\setminus W}}(-1)^{|T|}g[W]\\\\\n",
    "g[S] = \\sum_{T\\subseteq S}(-1)^{|T|}\\sum_{W\\subseteq {S\\setminus T}}g[W]\\\\\n",
    "g[S] = \\sum_{T\\subseteq S}(-1)^{|T|}g[S\\setminus T]\\\\\n",
    "g[S] = \\sum_{T\\subseteq S}(-1)^{|S|-|T|}g[T]\\\\\n",
    "Q.E.D.$\n",
    "\n",
    "## 单位根反演\n",
    "\n",
    "### Core formula\n",
    "\n",
    "$\\omega_n$: $n$次单位根 s.t. $\\omega_n^n=1$ (e.g. 复数域上的$e^{\\frac{2\\pi i}{n}}$).\n",
    "\n",
    "$\\frac{1}{n}\\sum_{k=0}^{n-1}\\omega_n^{vk} = [v\\equiv 0\\mod n]$\n",
    "\n",
    "Given $f[m]=\\sum_{k=0}^{n-1}\\omega_n^{mk}g[k]$, we have:\n",
    "\n",
    "$g[m]=\\frac{1}{n}\\sum_{k=0}^{n-1}\\omega_n^{-mk}f[k]$.\n",
    "\n",
    "# Reference\n",
    "[炫酷反演魔术](https://vfleaking.blog.uoj.ac/blog/87)"
   ]
  }
 ],
 "metadata": {
  "kernelspec": {
   "display_name": "Python 3",
   "language": "python",
   "name": "python3"
  },
  "language_info": {
   "codemirror_mode": {
    "name": "ipython",
    "version": 3
   },
   "file_extension": ".py",
   "mimetype": "text/x-python",
   "name": "python",
   "nbconvert_exporter": "python",
   "pygments_lexer": "ipython3",
   "version": "3.8.5"
  }
 },
 "nbformat": 4,
 "nbformat_minor": 5
}
